Lp2lc/Active/LC/Def.lean
@@ -1,0 +1,47 @@
+import Mathlib.Tactic
+import «Lp2lc».Active.Shared
+import «Lp2lc».Util
+
+namespace Lp2lc.Active
+
+
+namespace LC -- untyped lambda calculus
+
+inductive AST(F: Rep) : Rep
+| bvar : Nat -> AST F .trm -- de Bruijn for bounded variable (TODO: marked for removal in PHOAS version)
+| fvar : Var -> AST F .trm -- name for free variable (they also have de Bruijn but are quite useless)
+| fn : (I: F .typ) -> (out: F .trm) -> AST F .trm -- {x: I => out}, out may contain x
+| app : (fn: F .trm) -> (x: F .trm) -> AST F .trm -- {fn(x)}
+| anyT : AST F .typ -- can bind anything, in type system without subtyping (e.g. LEAN, Haskell) this is usually an internal feature, user cannot declare it
+
+def Trm (F: Rep) := AST F .trm
+def Typ (F: Rep) := AST F .typ
+
+def EnvTrms (F: Rep) := Finset (Var × AST F .trm)
+def EnvTyps (F: Rep) := Finset (Var × AST F .typ)
+def Env (F: Rep) := EnvTrms F × EnvTyps F
+
+def typing (F: Rep) : Env F -> (x: Trm F) -> (T: Typ F) -> Prop -- true if x can inhabit T
+ := sorry
+
+def isValue : Trm F -> Prop
+  := sorry
+
+def canReduce : Trm F -> Trm F -> Prop
+  := sorry
+
+
+def preservation : Prop := ∀ (F: Rep) (E : Env F) (e e' : Trm F) (T : Typ F),
+  typing F E e T ->
+  canReduce e e' ->
+  typing F E e' T
+
+-- def progress : Prop := ∀ (F: Rep) (E: Env F) (e : Trm F) (T : Typ F),
+--   Typing E e T ->
+--   Value e ∨ (∃ e', Red e e')
+
+
+
+end LC
+
+end Lp2lc.Active
