Lp2lc/Active/STLC.lean
@@ -1,2 +1,4 @@
-import «Lp2lc».Active.STLC.StepIndexedDemo
-import «Lp2lc».Active.STLC.StepIndexDemo_partiallyCorrect
+-- STLC module exports Def and Example
+import «Lp2lc».Active.LC.Def
+import «Lp2lc».Active.STLC.Def
+import «Lp2lc».Active.STLC.Example
