Lp2lc/Active/STLC/Scratch.lean
@@ -1,0 +1,35 @@
+
+example : Type 1 := Type
+example : Type 1 := Type -> Type
+
+inductive Box0 (T : Type) : Type where
+  | mk : (v: T) -> Box0 T
+
+inductive Box1 : (T: Type) -> Type where
+  | mk : {T: Type} -> (v: T) -> Box1 T
+
+inductive Box3 : Type 1 where
+  | mk : {T: Type} -> (v: T) -> Box3
+def Box3AlsoMk {T: Type} (v: T) : Box3 := Box3.mk v
+
+inductive Box4 : Type 1 where
+  | mk {T: Type} : (v: T) -> Box4
+def Box4AlsoMk {T: Type} (v: T) : Box4 := Box4.mk v
+
+example : {T : Type} -> T -> Box3 := Box3.mk
+example : {T : Type} -> T -> Box3 := Box3AlsoMk
+example : {T : Type} -> T -> Box4 := Box4.mk
+example : {T : Type} -> T -> Box4 := Box4AlsoMk
+
+inductive Sys (typ: Type) (trm: Type) : Type where
+| mk : Sys typ trm
+
+
+example : Type -> Type -> Type := Sys
+
+
+-- structure Sys2 where
+--   typ: Type
+--   trm: Type
+
+-- example: Type -> Type -> Type := Sys2
