Lp2lc/Active/STLCv3_unsafe_sys/Def.lean
@@ -1,0 +1,114 @@
+import Mathlib.Tactic
+import «Lp2lc».Active.Shared
+
+namespace Lp2lc.Active
+
+-- System extension, induction rule always cast input into output in either the same system or the most specific system that defined the rule
+-- AKA, Typ and Trm are always closed under rules/composition/induction
+-- e.g. using STLC rule can cast STLC Typ into STLC Typ, or F Typ into F Typ
+-- but using F rule can only cast both STLC/F Typ into F Typ
+-- this goes both ways
+-- the problem is that theorems are defined for types (including wrapper), not rules
+-- Basic (pre)types --
+
+structure Sys : Type 1 where
+  FType: Type -- F stands for "fixed-point"
+  FTerm: Type
+
+namespace LC -- untyped lambda calculus
+
+inductive Trm (sys: Sys) : Type
+| bvar : Nat -> Trm sys -- de Bruijn for bounded variable
+| fvar : Var -> Trm sys -- name for free variable (they also have de Bruijn but are quite useless)
+| abs : (T: sys.FType) -> (x: sys.FTerm) -> Trm sys -- {x: T => x + 1}
+| app : (fn: sys.FTerm) -> (x: sys.FTerm) -> Trm sys -- {fn(x)}
+
+inductive Typ (sys: Sys) : Type
+| any : Typ sys -- can bind anything, in type system without subtyping (e.g. LEAN, Haskell) this is usually an internal feature not exposed to user
+deriving Repr
+
+end LC
+
+namespace STLC -- simply-typed lambda calculus
+
+abbrev Trm (sys: Sys) := LC.Trm sys
+
+inductive Typ (sys: Sys): Type
+| backbone: LC.Typ sys -> Typ sys -- unfold ([a] expression to its parts) should be free (cost no fuel) in induction, but no problem if it cost 1 fuel
+| arrow : sys.FType -> sys.FType -> (Typ sys)
+
+namespace Example
+
+  abbrev mk_sys (FType FTerm : Type) : Sys := {
+    FType := FType
+    FTerm := FTerm
+  }
+
+  mutual
+    unsafe structure RealTyp : Type where
+      self: Typ (mk_sys RealTyp RealTrm)
+
+    unsafe structure RealTrm : Type where
+      self: Trm (mk_sys RealTyp RealTrm)
+  end
+
+  unsafe def sys : Sys := mk_sys RealTyp RealTrm
+
+
+--   -- real expressions of RealTyp in STLC
+--   example :=
+--     let k1 :=  (any : LC.Typ RealTyp) -- LC
+--     let k2 := -- STLC(LC)
+--       let k1View : Typ RealTyp := Typ.backbone k1
+--       Typ.arrow (RealTyp.mk k1View) (RealTyp.mk k1View)
+--     let _ : RealTyp := RealTyp.mk k2 -- fixpoint of STLC(LC)
+--     Unit
+
+--   -- more generic STLC expressions in any type system that uses STLC as backbone
+--   -- namely, mk ensures that Typ F always has a representation in F
+--   -- the reverse (F -> Typ F) is not true (e.g. for System F)
+
+--   -- consequently, generic, extendable inductive proof need stronger conditions
+--   -- see Example in SysF for what these conditions look like
+--   example (F: Type) (mk: Typ F -> F) :=
+--     let k1 :=  (any : LC.Typ (F)) -- LC
+--     let k2 := -- STLC(LC)
+--       let _k1 : Typ F := Typ.backbone k1
+--       Typ.arrow (mk _k1) (mk _k1)
+--     let _ : F := mk k2 -- fixpoint of STLC(LC)
+--     Unit
+
+
+--   structure RealTrm where
+--     self: Trm RealTyp RealTrm
+--   deriving Repr
+
+--   example (mkT : Trm RealTyp RealTrm -> RealTrm) (mkY : Typ RealTyp -> RealTyp) :=
+--     let t1 := (any : LC.Typ RealTyp)
+--     let k1 := mkY (Typ.backbone t1)
+--     let e1 := (LC.Trm.abs k1 (mkT (Trm.backbone (LC.Trm.bvar 0))) : LC.Trm RealTyp RealTrm)
+--     let e2 := Trm.backbone e1
+--     let _ : RealTrm := mkT e2
+--     Unit
+
+end Example
+
+end STLC
+
+-- namespace SysF
+
+-- inductive Typ (F: Type): Type
+-- | backbone: STLC.Typ F -> Typ F
+-- | bvar : Nat -> Typ F -- binded type variable by De-Bruijn index
+-- | fvar : Var -> Typ F -- free type variable by name
+-- deriving Repr
+
+-- inductive Trm (F: Type) (G: Type) : Type
+-- | backbone : STLC.Trm F G -> Trm F G
+-- | tabs : F -> G -> Trm F G
+-- | tapp : G -> F -> Trm F G
+-- deriving Repr
+
+-- end SysF
+
+end Lp2lc.Active
