Lp2lc/Active/SysF/Def.lean
@@ -1,11 +1,18 @@
 import Mathlib.Tactic
 
 import «Lp2lc».Active.Shared
-import «Lp2lc».Active.STLC
+import «Lp2lc».Active.STLC.Def
 
 namespace Lp2lc.Active
 
 namespace SysF
+
+inductive AST(F: Rep) : Rep
+| backbone : {w : Which} -> STLC.AST F w -> AST F w
+| polyFn : (I: F .typ) -> (out: F .trm) -> AST F .trm -- polymorphic function {[I] => out}, out may contain I
+| polyApp : (poly: F .trm) -> (X: F .typ) -> AST F .trm -- apply polymorphic function {poly[X]}
+| bvarT : Nat -> AST F .typ -- like bvar, but for type
+| fvarT : Var -> AST F .typ -- like fvar, but for type
 
 end SysF
 
