Lp2lc/Util.lean
@@ -1,0 +1,1 @@
+import «Lp2lc».Util.Rfl
