Lp2lc/Util/Rfl.lean
@@ -1,0 +1,44 @@
+import Lean
+
+open Lean Elab Command Meta
+
+private partial def normalize_expr (e : Expr) : MetaM Expr := do
+  let e ← whnfR e
+  match e with
+  | .lam n d b bi =>
+      let d ← normalize_expr d
+      withLocalDecl n bi d fun x => do
+        let b ← normalize_expr (b.instantiate1 x)
+        mkLambdaFVars #[x] b
+  | .forallE n d b bi =>
+      let d ← normalize_expr d
+      withLocalDecl n bi d fun x => do
+        let b ← normalize_expr (b.instantiate1 x)
+        mkForallFVars #[x] b
+  | _ =>
+      reduceAll e
+
+syntax (name := rflCmd) "#rfl " term : command
+
+@[command_elab rflCmd] def elab_rfl_cmd : CommandElab
+  | `(#rfl $t:term) =>
+      withoutModifyingEnv <| runTermElabM fun _ =>
+        Term.withDeclName `_rfl do
+          let lhs ← Term.elabTerm t none
+          Term.synthesizeSyntheticMVarsNoPostponing
+          withRef t <| Meta.check lhs
+          let lhs ← Term.levelMVarToParam (← instantiateMVars lhs)
+          let rhs_source ←
+            match lhs with
+            | .const decl_name us =>
+                let info ← getConstInfo decl_name
+                match info.value? with
+                | some _ => instantiateValueLevelParams info us
+                | none => pure lhs
+            | _ =>
+                pure lhs
+          let rhs ← withTransparency (mode := .all) <| normalize_expr rhs_source
+          let lhs_fmt ← ppExpr lhs
+          let rhs_fmt ← ppExpr rhs
+          logInfoAt t m!"{lhs_fmt} = {rhs_fmt}"
+  | _ => throwUnsupportedSyntax
